@prefix : <http://www.semanticweb.org/alecsculley/ontologies/2025/3/untitled-ontology-113/> .
@prefix owl: <http://www.w3.org/2002/07/owl#> .
@prefix rdf: <http://www.w3.org/1999/02/22-rdf-syntax-ns#> .
@prefix xml: <http://www.w3.org/XML/1998/namespace> .
@prefix xsd: <http://www.w3.org/2001/XMLSchema#> .
@prefix rdfs: <http://www.w3.org/2000/01/rdf-schema#> .
@base <http://www.semanticweb.org/alecsculley/ontologies/2025/3/untitled-ontology-113/> .

<http://www.semanticweb.org/alecsculley/ontologies/2025/3/untitled-ontology-113> rdf:type owl:Ontology ;
                                                                                  owl:imports <https://www.commoncoreontologies.org/2024-11-06/CommonCoreOntologiesMerged> .

#################################################################
#    Annotation properties
#################################################################

###  http://www.w3.org/2004/02/skos/core#altLabel
<http://www.w3.org/2004/02/skos/core#altLabel> rdf:type owl:AnnotationProperty .


###  http://www.w3.org/2004/02/skos/core#definition
<http://www.w3.org/2004/02/skos/core#definition> rdf:type owl:AnnotationProperty .


#################################################################
#    Object Properties
#################################################################

###  http://www.semanticweb.org/alecsculley/ontologies/2025/3/untitled-ontology-113/backedBy
:backedBy rdf:type owl:ObjectProperty ;
          rdfs:label "backed by"@en ;
          <http://www.w3.org/2004/02/skos/core#definition> "x backed by y means x is supported, secured, or guaranteed by y, meaning that the value, performance, or repayment of x is underpinned by y."@en .


###  http://www.semanticweb.org/alecsculley/ontologies/2025/3/untitled-ontology-113/issues
:issues rdf:type owl:ObjectProperty ;
        rdfs:label "issues"@en .


###  http://www.semanticweb.org/alecsculley/ontologies/2025/3/untitled-ontology-113/partOf
:partOf rdf:type owl:ObjectProperty ;
        rdfs:label "part of"@en .


###  http://www.semanticweb.org/alecsculley/ontologies/2025/3/untitled-ontology-113/raisedBy
:raisedBy rdf:type owl:ObjectProperty ;
          rdfs:label "raised by"@en ;
          <http://www.w3.org/2004/02/skos/core#definition> "x raised by y means x is some resource, y is some agent, and x has been generated, collected, or acquired through the fundraising or financing efforts of y."@en .


#################################################################
#    Classes
#################################################################

###  http://www.semanticweb.org/alecsculley/ontologies/2025/3/untitled-ontology-113#12-Month_Time_Period
<http://www.semanticweb.org/alecsculley/ontologies/2025/3/untitled-ontology-113#12-Month_Time_Period> rdf:type owl:Class ;
                                                                                                      rdfs:subClassOf :Time_Period ;
                                                                                                      rdfs:label "12-Month Time Period"@en ;
                                                                                                      <http://www.w3.org/2004/02/skos/core#definition> "A continuous span of 12 consecutive months used as a standard benchmark for assessing performance or compliance."@en .


###  http://www.semanticweb.org/alecsculley/ontologies/2025/3/untitled-ontology-113#90-Day_Time_Period
<http://www.semanticweb.org/alecsculley/ontologies/2025/3/untitled-ontology-113#90-Day_Time_Period> rdf:type owl:Class ;
                                                                                                    rdfs:subClassOf :Time_Period ;
                                                                                                    rdfs:label "90-Day Time Period"@en .


###  http://www.semanticweb.org/alecsculley/ontologies/2025/3/untitled-ontology-113/AccreditedInvestorRole
:AccreditedInvestorRole rdf:type owl:Class ;
                        rdfs:subClassOf :Investor_Role ;
                        rdfs:label "Accredited Investor Role"@en ;
                        <http://www.w3.org/2004/02/skos/core#definition> "An investor role that inheres in an agent in virtue of that agent meeting certain requirements set by regulatory authorities."@en .


###  http://www.semanticweb.org/alecsculley/ontologies/2025/3/untitled-ontology-113/Annual_Income
:Annual_Income rdf:type owl:Class ;
               rdfs:subClassOf <http://www.sks.ai/ont/SumOfMoney> ;
               rdfs:label "Annual Income"@en ;
               <http://www.w3.org/2004/02/skos/core#definition> "The sum of money that an agent earns in a year."@en .


###  http://www.semanticweb.org/alecsculley/ontologies/2025/3/untitled-ontology-113/Asset
:Asset rdf:type owl:Class ;
       rdfs:subClassOf <https://www.commoncoreontologies.org/ont00000740> ;
       rdfs:label "Asset"@en ;
       <http://www.w3.org/2004/02/skos/core#definition> "An Asset is a Resource that has economic value and is expected to generate future financial benefits."@en .


###  http://www.semanticweb.org/alecsculley/ontologies/2025/3/untitled-ontology-113/Bad_Actor
:Bad_Actor rdf:type owl:Class ;
           owl:equivalentClass [ owl:intersectionOf ( <https://www.commoncoreontologies.org/ont00001017>
                                                      [ rdf:type owl:Restriction ;
                                                        owl:onProperty <http://purl.obolibrary.org/obo/BFO_0000196> ;
                                                        owl:someValuesFrom :Bad_Actor_Role
                                                      ]
                                                    ) ;
                                 rdf:type owl:Class
                               ] ;
           rdfs:subClassOf <https://www.commoncoreontologies.org/ont00001017> ;
           rdfs:label "Bad Actor"@en ;
           <http://www.w3.org/2004/02/skos/core#definition> "An agent that is bearer of some bad actor role."@en .


###  http://www.semanticweb.org/alecsculley/ontologies/2025/3/untitled-ontology-113/Bad_Actor_Role
:Bad_Actor_Role rdf:type owl:Class ;
                rdfs:subClassOf <http://purl.obolibrary.org/obo/BFO_0000023> ;
                rdfs:label "Bad Actor Role"@en ;
                <http://www.w3.org/2004/02/skos/core#definition> "A role that inheres in an agent in virtue of their being disqualified from certain securities exemptions due to specified regulatory, criminal, or civil violations, and, if realized, is realized in some act the agent is disqualified from because of their violations."@en .


###  http://www.semanticweb.org/alecsculley/ontologies/2025/3/untitled-ontology-113/Blank_Check_Company
:Blank_Check_Company rdf:type owl:Class ;
                     rdfs:subClassOf <https://folio.openlegalstandard.org/RDdgYa5ZbqVnS9aGrOwQu5h> ;
                     rdfs:label "Blank Check Company"@en ;
                     <http://www.w3.org/2004/02/skos/core#definition> "An incorporated organization that lacks a specific busniess plan or identified acquisition, often formed for future mergers or acquisitions."@en .


###  http://www.semanticweb.org/alecsculley/ontologies/2025/3/untitled-ontology-113/Business_Development_Company
:Business_Development_Company rdf:type owl:Class ;
                              rdfs:subClassOf :Registered_Investment_Company ;
                              rdfs:label "Business Development Company"@en ;
                              <http://www.w3.org/2004/02/skos/core#definition> "A registered investment company that invests in or assists small, developing, or financially distressed incorporated organizations."@en .


###  http://www.semanticweb.org/alecsculley/ontologies/2025/3/untitled-ontology-113/Canadian_Issuer
:Canadian_Issuer rdf:type owl:Class ;
                 owl:equivalentClass [ rdf:type owl:Restriction ;
                                       owl:onProperty <http://purl.obolibrary.org/obo/BFO_0000196> ;
                                       owl:someValuesFrom <http://www.sks.ai/ont/CanadianIssuerRole>
                                     ] ;
                 rdfs:subClassOf :Non-U.S._Issuer ;
                 rdfs:label "Canadian Issuer"@en ;
                 <http://www.w3.org/2004/02/skos/core#definition> "A non-US issuer that is bearer of some Canadian issuer role."@en .


###  http://www.semanticweb.org/alecsculley/ontologies/2025/3/untitled-ontology-113/Capital-Raising_Limit
:Capital-Raising_Limit rdf:type owl:Class ;
                       rdfs:subClassOf <https://www.commoncoreontologies.org/ont00000965> ;
                       rdfs:label "Capital-Raising Limit"@en ;
                       <http://www.w3.org/2004/02/skos/core#definition> "A directive information content entity that prescribes the amount of capital an issuer is permitted to raise within a particular temporal interval."@en .


###  http://www.semanticweb.org/alecsculley/ontologies/2025/3/untitled-ontology-113/DisclosureDocumentContent
:DisclosureDocumentContent rdf:type owl:Class ;
                           rdfs:subClassOf :LegalDocumentContent ;
                           owl:disjointWith :OfferingDocumentContent ;
                           rdfs:label "Disclosure Document Content"@en ;
                           <http://www.w3.org/2004/02/skos/core#definition> "A Legal Document Content that is provided by an issuer in connection with a securities offering and is about the offering, the issuer, the risks involved, and other factors necessary to enable investors to make informed investment decisions."@en .


###  http://www.semanticweb.org/alecsculley/ontologies/2025/3/untitled-ontology-113/Disclosure_Document
:Disclosure_Document rdf:type owl:Class ;
                     owl:equivalentClass [ owl:intersectionOf ( :Legal_Document
                                                                [ rdf:type owl:Restriction ;
                                                                  owl:onProperty <http://purl.obolibrary.org/obo/BFO_0000101> ;
                                                                  owl:someValuesFrom :DisclosureDocumentContent
                                                                ]
                                                              ) ;
                                           rdf:type owl:Class
                                         ] ;
                     rdfs:subClassOf :Legal_Document ;
                     rdfs:label "Disclosure Document"@en ;
                     <http://www.w3.org/2004/02/skos/core#definition> "A legal document that is carrier of some disclosure document content."@en .


###  http://www.semanticweb.org/alecsculley/ontologies/2025/3/untitled-ontology-113/Exchange_Act_Reporting_Company
:Exchange_Act_Reporting_Company rdf:type owl:Class ;
                                rdfs:subClassOf <https://folio.openlegalstandard.org/RDdgYa5ZbqVnS9aGrOwQu5h> ;
                                rdfs:label "Exchange Act Reporting Company"@en ;
                                <http://www.w3.org/2004/02/skos/core#definition> "An incorporated organization that is registered under the Securities Exchange Act of 1934 and files periodic reports with the SEC."@en .


###  http://www.semanticweb.org/alecsculley/ontologies/2025/3/untitled-ontology-113/Federal_Limit
:Federal_Limit rdf:type owl:Class ;
               rdfs:subClassOf :Offering_Limit ;
               rdfs:label "Federal Offering Limit"@en ;
               <http://www.w3.org/2004/02/skos/core#definition> "An offering limit prescribed by federal law."@en .


###  http://www.semanticweb.org/alecsculley/ontologies/2025/3/untitled-ontology-113/Form_C
:Form_C rdf:type owl:Class ;
        rdfs:subClassOf :Disclosure_Document ;
        rdfs:label "Form C"@en ;
        <http://www.w3.org/2004/02/skos/core#definition> "Form C is the disclosure document that an issuer must file with the SEC when conducting a securities offering under Regulation Crowdfunding, detailing the company’s business, financial condition, offering specifics, and intended use of proceeds to inform potential investors."@en .


###  http://www.semanticweb.org/alecsculley/ontologies/2025/3/untitled-ontology-113/General_Solicitation
:General_Solicitation rdf:type owl:Class ;
                      rdfs:subClassOf :Solicitation ;
                      rdfs:label "Act of General Solicitation"@en ;
                      <http://www.w3.org/2004/02/skos/core#definition> "An act of solicitation that targets the public broadly by using mass communication channels."@en .


###  http://www.semanticweb.org/alecsculley/ontologies/2025/3/untitled-ontology-113/In-State_Resident
:In-State_Resident rdf:type owl:Class ;
                   owl:equivalentClass [ rdf:type owl:Restriction ;
                                         owl:onProperty <http://purl.obolibrary.org/obo/BFO_0000196> ;
                                         owl:someValuesFrom <http://www.sks.ai/ont/InStateResidentRole>
                                       ] ;
                   rdfs:subClassOf <https://www.commoncoreontologies.org/ont00001017> ;
                   rdfs:label "In-State Resident"@en ;
                   <http://www.w3.org/2004/02/skos/core#definition> "An agent that is bearer of some in-state resident role."@en .


###  http://www.semanticweb.org/alecsculley/ontologies/2025/3/untitled-ontology-113/Internet_Platform
:Internet_Platform rdf:type owl:Class ;
                   rdfs:subClassOf <http://purl.obolibrary.org/obo/BFO_0000031> ;
                   rdfs:label "Internet Platform"@en ;
                   <http://www.w3.org/2004/02/skos/core#definition> "A generically dependent continuant that is a digital system or service that facilitates interactions, transactions, or content sharing between users or between users and applications, typically by providing a structured environment built on internet protocols."@en .


###  http://www.semanticweb.org/alecsculley/ontologies/2025/3/untitled-ontology-113/Investment_Company
:Investment_Company rdf:type owl:Class ;
                    rdfs:subClassOf <https://folio.openlegalstandard.org/RDdgYa5ZbqVnS9aGrOwQu5h> ;
                    rdfs:label "Investment Company"@en ;
                    <http://www.w3.org/2004/02/skos/core#definition> "An incorporated organization whose principal activity involves investing, holding, or trading securities."@en .


###  http://www.semanticweb.org/alecsculley/ontologies/2025/3/untitled-ontology-113/Investment_Limit
:Investment_Limit rdf:type owl:Class ;
                  rdfs:subClassOf :Capital-Raising_Limit ;
                  rdfs:label "Investment Limit"@en ;
                  <http://www.w3.org/2004/02/skos/core#definition> "A capital-raising limit that prescribes the amount of capital that a single investor is permitted to contribute to an offering."@en .


###  http://www.semanticweb.org/alecsculley/ontologies/2025/3/untitled-ontology-113/Investor_Role
:Investor_Role rdf:type owl:Class ;
               rdfs:subClassOf <http://purl.obolibrary.org/obo/BFO_0000023> ;
               rdfs:label "Investor Role"@en ;
               <http://www.w3.org/2004/02/skos/core#definition> "A role that inheres in an agent in virtue of that agent allocating financial capital with the expectation of future returns, and, if realized, is realized in an act of investment."@en .


###  http://www.semanticweb.org/alecsculley/ontologies/2025/3/untitled-ontology-113/Issuer_Role
:Issuer_Role rdf:type owl:Class ;
             rdfs:subClassOf <http://purl.obolibrary.org/obo/BFO_0000023> ;
             rdfs:label "Issuer Role"@en ;
             <http://www.w3.org/2004/02/skos/core#definition> "A role that inheres in an agent in virtue of developing, registering, and selling securities to finance its operations, and, if realized, is realized  in an act of issuing securities."@en .


###  http://www.semanticweb.org/alecsculley/ontologies/2025/3/untitled-ontology-113/LegalDocumentContent
:LegalDocumentContent rdf:type owl:Class ;
                      owl:equivalentClass [ rdf:type owl:Restriction ;
                                            owl:onProperty <http://purl.obolibrary.org/obo/BFO_0000084> ;
                                            owl:someValuesFrom <https://www.commoncoreontologies.org/ont00001346>
                                          ] ;
                      rdfs:subClassOf <https://www.commoncoreontologies.org/ont00000958> ;
                      rdfs:label "Legal Document Content"@en ;
                      <http://www.w3.org/2004/02/skos/core#definition> "Information content entity that generically depends on some legal instrument."@en .


###  http://www.semanticweb.org/alecsculley/ontologies/2025/3/untitled-ontology-113/Legal_Document
:Legal_Document rdf:type owl:Class ;
                owl:equivalentClass [ owl:intersectionOf ( <https://www.commoncoreontologies.org/ont00001298>
                                                           [ rdf:type owl:Restriction ;
                                                             owl:onProperty <http://purl.obolibrary.org/obo/BFO_0000101> ;
                                                             owl:someValuesFrom :LegalDocumentContent
                                                           ]
                                                         ) ;
                                      rdf:type owl:Class
                                    ] ;
                rdfs:subClassOf <https://www.commoncoreontologies.org/ont00001298> ;
                rdfs:label "Legal Document"@en ;
                <http://www.w3.org/2004/02/skos/core#definition> "A document that is carrier of some legal document content."@en .


###  http://www.semanticweb.org/alecsculley/ontologies/2025/3/untitled-ontology-113/Net_Worth
:Net_Worth rdf:type owl:Class ;
           rdfs:subClassOf <https://www.commoncoreontologies.org/ont00001364> ;
           rdfs:label "Net Worth"@en ;
           <http://www.w3.org/2004/02/skos/core#definition> "An interval measurement information content entity that measures the value of an agent's assets minus that agent's liabilities."@en .


###  http://www.semanticweb.org/alecsculley/ontologies/2025/3/untitled-ontology-113/Non-Accredited_Investor
:Non-Accredited_Investor rdf:type owl:Class ;
                         owl:equivalentClass [ owl:intersectionOf ( <https://folio.openlegalstandard.org/R8hWq9dSn0Su2Y59JE48V3H>
                                                                    [ rdf:type owl:Class ;
                                                                      owl:complementOf [ rdf:type owl:Restriction ;
                                                                                         owl:onProperty <http://purl.obolibrary.org/obo/BFO_0000196> ;
                                                                                         owl:someValuesFrom :AccreditedInvestorRole
                                                                                       ]
                                                                    ]
                                                                  ) ;
                                               rdf:type owl:Class
                                             ] ;
                         rdfs:subClassOf <https://folio.openlegalstandard.org/R8hWq9dSn0Su2Y59JE48V3H> ;
                         owl:disjointWith <https://folio.openlegalstandard.org/RCwEVoFW90PLN1eL6JToOMt> ;
                         rdfs:label "Non-Accredited Investor"@en ;
                         <http://www.w3.org/2004/02/skos/core#definition> "An investor and is not bearer of some accredited investor role."@en .


###  http://www.semanticweb.org/alecsculley/ontologies/2025/3/untitled-ontology-113/Non-U.S._Issuer
:Non-U.S._Issuer rdf:type owl:Class ;
                 owl:equivalentClass [ rdf:type owl:Restriction ;
                                       owl:onProperty <http://purl.obolibrary.org/obo/BFO_0000196> ;
                                       owl:someValuesFrom <http://www.sks.ai/ont/NonUSIssuerRole>
                                     ] ;
                 rdfs:subClassOf <https://folio.openlegalstandard.org/RDM4k8t0O3hy93vQwQzEcpg> ;
                 rdfs:label "Non-U.S. Issuer"@en ;
                 <http://www.w3.org/2004/02/skos/core#definition> "An issuer that is bearer of some non-US issuer role."@en .


###  http://www.semanticweb.org/alecsculley/ontologies/2025/3/untitled-ontology-113/Offeree
:Offeree rdf:type owl:Class ;
         owl:equivalentClass [ owl:intersectionOf ( <https://www.commoncoreontologies.org/ont00001017>
                                                    [ rdf:type owl:Restriction ;
                                                      owl:onProperty <http://purl.obolibrary.org/obo/BFO_0000196> ;
                                                      owl:someValuesFrom :Offeree_Role
                                                    ]
                                                  ) ;
                               rdf:type owl:Class
                             ] ;
         rdfs:subClassOf <https://www.commoncoreontologies.org/ont00001017> ;
         rdfs:label "Offeree"@en ;
         <http://www.w3.org/2004/02/skos/core#definition> "An agent that is bearer of some offeree role."@en .


###  http://www.semanticweb.org/alecsculley/ontologies/2025/3/untitled-ontology-113/Offeree_Role
:Offeree_Role rdf:type owl:Class ;
              rdfs:subClassOf <http://purl.obolibrary.org/obo/BFO_0000023> ;
              rdfs:label "Offeree Role"@en ;
              <http://www.w3.org/2004/02/skos/core#definition> "A role that inheres in an Aqgent in virtue of that agent being extended an offer to purchase securities, and, if realized, is realized in in an act of  being offered an opprotunity to purchase securities."@en .


###  http://www.semanticweb.org/alecsculley/ontologies/2025/3/untitled-ontology-113/OfferingDocumentContent
:OfferingDocumentContent rdf:type owl:Class ;
                         rdfs:subClassOf :LegalDocumentContent ;
                         rdfs:label "Offering Document Content"@en ;
                         <http://www.w3.org/2004/02/skos/core#definition> "A legal document content provided by a company or financial entity to potential investors, detailing the terms, conditions, and risks of the investment offering."@en .


###  http://www.semanticweb.org/alecsculley/ontologies/2025/3/untitled-ontology-113/Offering_Limit
:Offering_Limit rdf:type owl:Class ;
                rdfs:subClassOf :Capital-Raising_Limit ;
                rdfs:label "Offering Limit"@en ;
                <http://www.w3.org/2004/02/skos/core#definition> "A capital-raisinf limit that prescribes the amount of capital that an issuer can raise within a particular temporal interval."@en .


###  http://www.semanticweb.org/alecsculley/ontologies/2025/3/untitled-ontology-113/Process_of_Issuing_Securities
:Process_of_Issuing_Securities rdf:type owl:Class ;
                               rdfs:subClassOf <https://www.commoncoreontologies.org/ont00001314> ;
                               rdfs:label "Act of Issuing Securities"@en ;
                               <http://www.w3.org/2004/02/skos/core#definition> "A legal system act in which an agent creates, registers, and offers its financial instruments to investors."@en .


###  http://www.semanticweb.org/alecsculley/ontologies/2025/3/untitled-ontology-113/Process_of_Testing_the_Waters
:Process_of_Testing_the_Waters rdf:type owl:Class ;
                               rdfs:subClassOf <https://www.commoncoreontologies.org/ont00000402> ;
                               rdfs:label "Act of Testing the Waters"@en ;
                               <http://www.w3.org/2004/02/skos/core#definition> "An act of communication in which an issuer engages potential investors before formally committing to an offering."@en .


###  http://www.semanticweb.org/alecsculley/ontologies/2025/3/untitled-ontology-113/Process_of_Transaction
:Process_of_Transaction rdf:type owl:Class ;
                        rdfs:subClassOf <https://www.commoncoreontologies.org/ont00000433> ;
                        rdfs:label "Act of Transacting"@en ;
                        <http://www.w3.org/2004/02/skos/core#definition> "A planned act in which agents exchange entities of economic value."@en .


###  http://www.semanticweb.org/alecsculley/ontologies/2025/3/untitled-ontology-113/Qualification
:Qualification rdf:type owl:Class ;
               rdfs:subClassOf <https://www.commoncoreontologies.org/ont00001314> ;
               rdfs:label "Act of Qualificaiton"@en ;
               <http://www.w3.org/2004/02/skos/core#altLabel> "Qualification"@en ;
               <http://www.w3.org/2004/02/skos/core#definition> "A legal system act in which a securities authority declares that an offering document meets the legal requirements."@en .


###  http://www.semanticweb.org/alecsculley/ontologies/2025/3/untitled-ontology-113/Raised_Capital
:Raised_Capital rdf:type owl:Class ;
                rdfs:subClassOf <https://folio.openlegalstandard.org/RxkTKgYqWS0WBHnJgrn27Y> ;
                rdfs:label "Raised Capital"@en ;
                <http://www.w3.org/2004/02/skos/core#definition> "A financial asset a company secures by issuing securities to external investors, which then become part of its capital for operations and growth."@en .


###  http://www.semanticweb.org/alecsculley/ontologies/2025/3/untitled-ontology-113/Registered_Intermediary
:Registered_Intermediary rdf:type owl:Class ;
                         owl:equivalentClass [ owl:intersectionOf ( <https://www.commoncoreontologies.org/ont00001017>
                                                                    [ rdf:type owl:Restriction ;
                                                                      owl:onProperty <http://purl.obolibrary.org/obo/BFO_0000196> ;
                                                                      owl:someValuesFrom :Registered_Intermediary_Role
                                                                    ]
                                                                  ) ;
                                               rdf:type owl:Class
                                             ] ;
                         rdfs:subClassOf <https://www.commoncoreontologies.org/ont00001017> ;
                         rdfs:label "Registered Intermediary"@en ;
                         <http://www.w3.org/2004/02/skos/core#definition> "An agent that is bearer of some registered intermediary role."@en .


###  http://www.semanticweb.org/alecsculley/ontologies/2025/3/untitled-ontology-113/Registered_Intermediary_Role
:Registered_Intermediary_Role rdf:type owl:Class ;
                              rdfs:subClassOf <http://purl.obolibrary.org/obo/BFO_0000023> ;
                              rdfs:label "Registered Intermediary Role"@en ;
                              <http://www.w3.org/2004/02/skos/core#definition> "A role that inheres in an agent in virtue of that agent being formally registered with a regulatory authority to act as a trusted agent between parties in financial transactions, ensuring compliance with applicable laws and regulations, and, if realized, is realized in an act of the correlated type."@en .


###  http://www.semanticweb.org/alecsculley/ontologies/2025/3/untitled-ontology-113/Registered_Investment_Company
:Registered_Investment_Company rdf:type owl:Class ;
                               rdfs:subClassOf :Investment_Company ;
                               rdfs:label "Registered Investment Company"@en ;
                               <http://www.w3.org/2004/02/skos/core#definition> "An investment company that has formally registered under the Investment Company Act of 1940."@en .


###  http://www.semanticweb.org/alecsculley/ontologies/2025/3/untitled-ontology-113/Security
:Security rdf:type owl:Class ;
          rdfs:subClassOf <https://folio.openlegalstandard.org/RxkTKgYqWS0WBHnJgrn27Y> ;
          rdfs:label "Security"@en ;
          <http://www.w3.org/2004/02/skos/core#definition> "A financial asset that represents an ownership interest, creditor relationship, or rights to potential future value."@en .


###  http://www.semanticweb.org/alecsculley/ontologies/2025/3/untitled-ontology-113/Solicitation
:Solicitation rdf:type owl:Class ;
              rdfs:subClassOf <https://www.commoncoreontologies.org/ont00000402> ,
                              [ rdf:type owl:Restriction ;
                                owl:onProperty :partOf ;
                                owl:someValuesFrom :Process_of_Issuing_Securities
                              ] ;
              rdfs:label "Act of Solicitation"@en ;
              <http://www.w3.org/2004/02/skos/core#definition> "An act of communication in which an issuer, or agent of an issuer, seeks to attract potential investors to purchase securities."@en .


###  http://www.semanticweb.org/alecsculley/ontologies/2025/3/untitled-ontology-113/Sophisticated_Investor
:Sophisticated_Investor rdf:type owl:Class ;
                        owl:equivalentClass [ rdf:type owl:Restriction ;
                                              owl:onProperty <http://purl.obolibrary.org/obo/BFO_0000196> ;
                                              owl:someValuesFrom <http://www.sks.ai/ont/SophisticatedInvestorRole>
                                            ] ;
                        rdfs:subClassOf <https://folio.openlegalstandard.org/R8hWq9dSn0Su2Y59JE48V3H> ;
                        rdfs:label "Sophisticated Investor"@en ;
                        <http://www.w3.org/2004/02/skos/core#definition> "An agent that is bearer of some sophisticated investor role."@en .


###  http://www.semanticweb.org/alecsculley/ontologies/2025/3/untitled-ontology-113/State_Limit
:State_Limit rdf:type owl:Class ;
             rdfs:subClassOf :Offering_Limit ;
             rdfs:label "State Offering Limit"@en ;
             <http://www.w3.org/2004/02/skos/core#definition> "An offering limit prescribed by state law."@en .


###  http://www.semanticweb.org/alecsculley/ontologies/2025/3/untitled-ontology-113/Time_Period
:Time_Period rdf:type owl:Class ;
             rdfs:subClassOf <http://purl.obolibrary.org/obo/BFO_0000202> ;
             rdfs:label "Time Period"@en ;
             <http://www.w3.org/2004/02/skos/core#definition> "A defined interval during which a particular event occurs."@en .


###  http://www.semanticweb.org/alecsculley/ontologies/2025/3/untitled-ontology-113/U.S._Issuer
:U.S._Issuer rdf:type owl:Class ;
             owl:equivalentClass [ rdf:type owl:Restriction ;
                                   owl:onProperty <http://purl.obolibrary.org/obo/BFO_0000196> ;
                                   owl:someValuesFrom <http://www.sks.ai/ont/USIssuerRole>
                                 ] ;
             rdfs:subClassOf <https://folio.openlegalstandard.org/RDM4k8t0O3hy93vQwQzEcpg> ;
             rdfs:label "U.S. Issuer"@en ;
             <http://www.w3.org/2004/02/skos/core#definition> "An issuer that is bearer of some US issuer role."@en .


###  http://www.sks.ai/ont/ActOfBusiness
<http://www.sks.ai/ont/ActOfBusiness> rdf:type owl:Class ;
                                      rdfs:subClassOf :Process_of_Transaction ;
                                      rdfs:label "Act of Business"@en ;
                                      <http://www.w3.org/2004/02/skos/core#definition> "An act of transacting that has agent some incorporated organization and is done to make profit."@en .


###  http://www.sks.ai/ont/ActOfInStateBusiness
<http://www.sks.ai/ont/ActOfInStateBusiness> rdf:type owl:Class ;
                                             rdfs:subClassOf <http://www.sks.ai/ont/ActOfBusiness> ;
                                             rdfs:label "Act of In-state Business"@en ;
                                             <http://www.w3.org/2004/02/skos/core#definition> "An act of business that occurs in some state and has agent some incorporated organization that either: (i) has a principal office and majority of employees or assets in that state; (ii) condusts a significant portion of revenue-generating activity in that state."@en .


###  http://www.sks.ai/ont/CanadianIssuerRole
<http://www.sks.ai/ont/CanadianIssuerRole> rdf:type owl:Class ;
                                           rdfs:subClassOf <http://www.sks.ai/ont/NonUSIssuerRole> ;
                                           rdfs:label "Canadian Issuer Role"@en ;
                                           <http://www.w3.org/2004/02/skos/core#definition> "A non-US issuer role that inheres in an agent in virtue of that agent being organized in, or maintaining its principal place of business in, Canada.en"@en .


###  http://www.sks.ai/ont/DisclosureDocument
<http://www.sks.ai/ont/DisclosureDocument> rdf:type owl:Class ;
                                           owl:equivalentClass [ rdf:type owl:Restriction ;
                                                                 owl:onProperty <http://purl.obolibrary.org/obo/BFO_0000101> ;
                                                                 owl:someValuesFrom :DisclosureDocumentContent
                                                               ] ;
                                           rdfs:subClassOf <https://www.commoncoreontologies.org/ont00001346> ;
                                           rdfs:label "Disclosure Document"@en ;
                                           <http://www.w3.org/2004/02/skos/core#definition> "A legal instrument that carries some disclosure document content."@en .


###  http://www.sks.ai/ont/FormC
<http://www.sks.ai/ont/FormC> rdf:type owl:Class ;
                              owl:equivalentClass [ rdf:type owl:Restriction ;
                                                    owl:onProperty <http://purl.obolibrary.org/obo/BFO_0000101> ;
                                                    owl:someValuesFrom <http://www.sks.ai/ont/FormCContent>
                                                  ] ;
                              rdfs:subClassOf <http://www.sks.ai/ont/DisclosureDocument> ;
                              rdfs:label "Form C"@en ;
                              <http://www.w3.org/2004/02/skos/core#definition> "A disclosure document that carries some Form C content."@en .


###  http://www.sks.ai/ont/FormCContent
<http://www.sks.ai/ont/FormCContent> rdf:type owl:Class ;
                                     rdfs:subClassOf :DisclosureDocumentContent ;
                                     rdfs:label "Form C Content"@en ;
                                     <http://www.w3.org/2004/02/skos/core#definition> "A disclosure document content that an issuer must file with the SEC when conducting a securities offering under Regulation Crowdfunding, detailing the company’s business, financial condition, offering specifics, and intended use of proceeds to inform potential investors."@en .


###  http://www.sks.ai/ont/FormD
<http://www.sks.ai/ont/FormD> rdf:type owl:Class ;
                              owl:equivalentClass [ rdf:type owl:Restriction ;
                                                    owl:onProperty <http://purl.obolibrary.org/obo/BFO_0000101> ;
                                                    owl:someValuesFrom <http://www.sks.ai/ont/FormDContent>
                                                  ] ;
                              rdfs:subClassOf <https://www.commoncoreontologies.org/ont00001346> ;
                              rdfs:label "Form D"@en ;
                              <http://www.w3.org/2004/02/skos/core#definition> "A legal instrument that carries some Form D Content."@en .


###  http://www.sks.ai/ont/FormDContent
<http://www.sks.ai/ont/FormDContent> rdf:type owl:Class ;
                                     rdfs:subClassOf :LegalDocumentContent ;
                                     rdfs:label "Form D Content"@en ;
                                     <http://www.w3.org/2004/02/skos/core#definition> "A legal document content that companies must file with the SEC after they sell securities without registration under Regulation D, containing key details about the offering and issuer."@en .


###  http://www.sks.ai/ont/InStateResidentRole
<http://www.sks.ai/ont/InStateResidentRole> rdf:type owl:Class ;
                                            rdfs:subClassOf <http://purl.obolibrary.org/obo/BFO_0000023> ;
                                            rdfs:label "In-state Resident Role"@en ;
                                            <http://www.w3.org/2004/02/skos/core#definition> "A role that inheres in an agent in virtue of that agent being legally domiciled or primarily located in a particular state."@en .


###  http://www.sks.ai/ont/NationalSecuritiesExchangeMarketplace
<http://www.sks.ai/ont/NationalSecuritiesExchangeMarketplace> rdf:type owl:Class ;
                                                              rdfs:subClassOf <http://www.sks.ai/ont/SecuritiesExchangeMarketplace> ;
                                                              rdfs:label "National Securities Exchange Marketplace"@en ;
                                                              <http://www.w3.org/2004/02/skos/core#definition> "A securities exchange marketplace registered with the SEC under Section 6 of the Securities Exchange Act of 1934."@en .


###  http://www.sks.ai/ont/NationalSecuritiesExchangeOrganization
<http://www.sks.ai/ont/NationalSecuritiesExchangeOrganization> rdf:type owl:Class ;
                                                               rdfs:subClassOf <http://www.sks.ai/ont/SecuritiesExchangeOrganization> ;
                                                               rdfs:label "National Securities Exchange Organization"@en ;
                                                               <http://www.w3.org/2004/02/skos/core#definition> "An organization that, in part or in full, operates, or assists in operating, a national securities exchange marketplace."@en .


###  http://www.sks.ai/ont/NonUSIssuerRole
<http://www.sks.ai/ont/NonUSIssuerRole> rdf:type owl:Class ;
                                        rdfs:subClassOf :Issuer_Role ;
                                        rdfs:label "Non-US Issuer Role"@en ;
                                        <http://www.w3.org/2004/02/skos/core#definition> "An issuer role that inheres in an agent in virtue of that agent being organized outside of, or maintaining its principal place of business outside of, the United States."@en .


###  http://www.sks.ai/ont/OfferingDocument
<http://www.sks.ai/ont/OfferingDocument> rdf:type owl:Class ;
                                         owl:equivalentClass [ rdf:type owl:Restriction ;
                                                               owl:onProperty <http://purl.obolibrary.org/obo/BFO_0000101> ;
                                                               owl:someValuesFrom :OfferingDocumentContent
                                                             ] ;
                                         rdfs:subClassOf <https://www.commoncoreontologies.org/ont00001346> ;
                                         rdfs:label "Offering Document"@en ;
                                         <http://www.w3.org/2004/02/skos/core#definition> "A legal instrument that carries some offering document content."@en .


###  http://www.sks.ai/ont/RestrictedSecurity
<http://www.sks.ai/ont/RestrictedSecurity> rdf:type owl:Class ;
                                           rdfs:subClassOf :Security ;
                                           rdfs:label "Restricted Security"@en ;
                                           <http://www.w3.org/2004/02/skos/core#definition> "A security aquired from an issuer during an act of transacting that does not have a public offering as a process part or as a cause."@en .


###  http://www.sks.ai/ont/Section12jOrderContent
<http://www.sks.ai/ont/Section12jOrderContent> rdf:type owl:Class ;
                                               rdfs:subClassOf <https://www.commoncoreontologies.org/ont00000965> ;
                                               rdfs:label "Section 12(j) Order Content"@en ;
                                               <http://www.w3.org/2004/02/skos/core#definition> "A Directive Information Content Entity that suspends or revokes the registration of a security due to violations of disclosure or filing requirements, and is issued under section 12(j) of the Excurities Exchange Act of 1934."@en .


###  http://www.sks.ai/ont/SecuritiesExchangeMarketplace
<http://www.sks.ai/ont/SecuritiesExchangeMarketplace> rdf:type owl:Class ;
                                                      rdfs:subClassOf <http://purl.obolibrary.org/obo/BFO_0000002> ;
                                                      rdfs:label "Securities Exchange Marketplace"@en ;
                                                      <http://www.w3.org/2004/02/skos/core#definition> "A marketplace where agents buy and sell securities."@en .


###  http://www.sks.ai/ont/SecuritiesExchangeOrganization
<http://www.sks.ai/ont/SecuritiesExchangeOrganization> rdf:type owl:Class ;
                                                       rdfs:subClassOf <https://www.commoncoreontologies.org/ont00001180> ;
                                                       rdfs:label "Securities Exchange Organization"@en ;
                                                       <http://www.w3.org/2004/02/skos/core#definition> "An organization that, in part or in full, operates, or assists in operating, a securities exchange marketplace."@en .


###  http://www.sks.ai/ont/SophisticatedInvestorRole
<http://www.sks.ai/ont/SophisticatedInvestorRole> rdf:type owl:Class ;
                                                  rdfs:subClassOf :Investor_Role ;
                                                  rdfs:label "Sophisticated Investor Role"@en ;
                                                  <http://www.w3.org/2004/02/skos/core#definition> "An investor role that inheres in an agent in virtue of qualifying under the Securities Act of 1933 and related Securities and Exchange Commission regulations as having sufficient knowledge and expertise in financial matters to weigh the value and risks of an investment."@en .


###  http://www.sks.ai/ont/SumOfMoney
<http://www.sks.ai/ont/SumOfMoney> rdf:type owl:Class ;
                                   rdfs:subClassOf <https://www.commoncoreontologies.org/ont00000740> ;
                                   rdfs:label "Sum of Money"@en ;
                                   <http://www.w3.org/2004/02/skos/core#definition> "A resource that is a collection of digital or physical money."@en .


###  http://www.sks.ai/ont/USIssuerRole
<http://www.sks.ai/ont/USIssuerRole> rdf:type owl:Class ;
                                     rdfs:subClassOf :Issuer_Role ;
                                     rdfs:label "US Issuer Role"@en ;
                                     <http://www.w3.org/2004/02/skos/core#definition> "An issuer role that inheres in an agent in virtue of that agent being organized in, or maintaining its principal place of business in, the United States."@en .


###  https://folio.openlegalstandard.org/R8hWq9dSn0Su2Y59JE48V3H
<https://folio.openlegalstandard.org/R8hWq9dSn0Su2Y59JE48V3H> rdf:type owl:Class ;
                                                              owl:equivalentClass [ owl:intersectionOf ( <https://www.commoncoreontologies.org/ont00001017>
                                                                                                         [ rdf:type owl:Restriction ;
                                                                                                           owl:onProperty <http://purl.obolibrary.org/obo/BFO_0000196> ;
                                                                                                           owl:someValuesFrom :Investor_Role
                                                                                                         ]
                                                                                                       ) ;
                                                                                    rdf:type owl:Class
                                                                                  ] ;
                                                              rdfs:subClassOf <https://www.commoncoreontologies.org/ont00001017> ;
                                                              rdfs:label "Investor"@en ;
                                                              <http://www.w3.org/2004/02/skos/core#definition> "An agent that is bearer of some investor role."@en .


###  https://folio.openlegalstandard.org/RBGd796pNg5ltGWhkyk2ifm
<https://folio.openlegalstandard.org/RBGd796pNg5ltGWhkyk2ifm> rdf:type owl:Class ;
                                                              owl:equivalentClass [ owl:intersectionOf ( :Security
                                                                                                         [ rdf:type owl:Restriction ;
                                                                                                           owl:onProperty :backedBy ;
                                                                                                           owl:someValuesFrom :Asset
                                                                                                         ]
                                                                                                       ) ;
                                                                                    rdf:type owl:Class
                                                                                  ] ;
                                                              rdfs:subClassOf :Security ;
                                                              rdfs:label "Asset-Backed Security"@en ;
                                                              <http://www.w3.org/2004/02/skos/core#definition> "A security backed by some asset."@en .


###  https://folio.openlegalstandard.org/RCwEVoFW90PLN1eL6JToOMt
<https://folio.openlegalstandard.org/RCwEVoFW90PLN1eL6JToOMt> rdf:type owl:Class ;
                                                              owl:equivalentClass [ owl:intersectionOf ( <https://folio.openlegalstandard.org/R8hWq9dSn0Su2Y59JE48V3H>
                                                                                                         [ rdf:type owl:Restriction ;
                                                                                                           owl:onProperty <http://purl.obolibrary.org/obo/BFO_0000196> ;
                                                                                                           owl:someValuesFrom :AccreditedInvestorRole
                                                                                                         ]
                                                                                                       ) ;
                                                                                    rdf:type owl:Class
                                                                                  ] ;
                                                              rdfs:subClassOf <https://folio.openlegalstandard.org/R8hWq9dSn0Su2Y59JE48V3H> ;
                                                              rdfs:label "Accredited Investor"@en ;
                                                              <http://www.w3.org/2004/02/skos/core#definition> "An investor that is bearer of some accredited investor role."@en .


###  https://folio.openlegalstandard.org/RDM4k8t0O3hy93vQwQzEcpg
<https://folio.openlegalstandard.org/RDM4k8t0O3hy93vQwQzEcpg> rdf:type owl:Class ;
                                                              owl:equivalentClass [ owl:intersectionOf ( <https://www.commoncoreontologies.org/ont00001017>
                                                                                                         [ rdf:type owl:Restriction ;
                                                                                                           owl:onProperty <http://purl.obolibrary.org/obo/BFO_0000196> ;
                                                                                                           owl:someValuesFrom :Issuer_Role
                                                                                                         ]
                                                                                                       ) ;
                                                                                    rdf:type owl:Class
                                                                                  ] ;
                                                              rdfs:subClassOf <https://www.commoncoreontologies.org/ont00001017> ;
                                                              rdfs:label "Issuer"@en ;
                                                              <http://www.w3.org/2004/02/skos/core#definition> "An issuer is a legal entity that develops, registers and sells securities to finance its operations. Issuers may be corporations, investment trusts, or domestic or foreign governments."@en .


###  https://folio.openlegalstandard.org/RDdgYa5ZbqVnS9aGrOwQu5h
<https://folio.openlegalstandard.org/RDdgYa5ZbqVnS9aGrOwQu5h> rdf:type owl:Class ;
                                                              owl:equivalentClass <https://www.commoncoreontologies.org/ont00000010> ;
                                                              rdfs:subClassOf <https://www.commoncoreontologies.org/ont00001180> ;
                                                              rdfs:label "Corporation"@en ;
                                                              <http://www.w3.org/2004/02/skos/core#altLabel> "Company"@en ;
                                                              <http://www.w3.org/2004/02/skos/core#definition> "An organization formed with state governmental approval to act as an artificial person that is empowered with legal rights usually only reserved for individuals, such as to sue and be sued, issue shares of stock to raise funds (unless it is non-profit), own property, hire employees or loan and borrow money."@en .


###  https://folio.openlegalstandard.org/RFLCbWnBgkHxPAEeVWloyg
<https://folio.openlegalstandard.org/RFLCbWnBgkHxPAEeVWloyg> rdf:type owl:Class ;
                                                             rdfs:subClassOf <https://www.commoncoreontologies.org/ont00001314> ;
                                                             rdfs:label "Act of Filing"@en ;
                                                             <http://www.w3.org/2004/02/skos/core#definition> "A legal system act that consists in the submission of a legal document that initiates some legal system act."@en .


###  https://folio.openlegalstandard.org/RmqysGFQ1RYW3F9lv5u3hu
<https://folio.openlegalstandard.org/RmqysGFQ1RYW3F9lv5u3hu> rdf:type owl:Class ;
                                                             rdfs:subClassOf :Legal_Document ;
                                                             rdfs:label "Offering Document"@en ;
                                                             <http://www.w3.org/2004/02/skos/core#altLabel> "Offering Statement"@en ;
                                                             <http://www.w3.org/2004/02/skos/core#definition> "A legal document that is carrier of some offering document content."@en .


###  https://folio.openlegalstandard.org/RxkTKgYqWS0WBHnJgrn27Y
<https://folio.openlegalstandard.org/RxkTKgYqWS0WBHnJgrn27Y> rdf:type owl:Class ;
                                                             rdfs:subClassOf :Asset ;
                                                             rdfs:label "Financial Asset"@en ;
                                                             <http://www.w3.org/2004/02/skos/core#altLabel> "Capital Resource"@en ;
                                                             <http://www.w3.org/2004/02/skos/core#definition> "An asset that has financial value, and which is expected to generate future financial benefits."@en .


###  https://www.commoncoreontologies.org/ont00000740
<https://www.commoncoreontologies.org/ont00000740> rdf:type owl:Class ;
                                                   rdfs:label "Resource"@en ;
                                                   <http://www.w3.org/2004/02/skos/core#definition> "A Continuant that is owned by, in the possession of, or is otherwise controlled by an Agent such that it could be used by that Agent."@en .


#################################################################
#    General axioms
#################################################################

[ rdf:type owl:AllDisjointClasses ;
  owl:members ( :Bad_Actor_Role
                :Investor_Role
                :Issuer_Role
                :Offeree_Role
                :Registered_Intermediary_Role
                <https://www.commoncoreontologies.org/ont00000038>
                <https://www.commoncoreontologies.org/ont00000173>
                <https://www.commoncoreontologies.org/ont00000175>
                <https://www.commoncoreontologies.org/ont00000187>
                <https://www.commoncoreontologies.org/ont00000392>
                <https://www.commoncoreontologies.org/ont00000485>
                <https://www.commoncoreontologies.org/ont00000506>
                <https://www.commoncoreontologies.org/ont00000599>
                <https://www.commoncoreontologies.org/ont00000758>
                <https://www.commoncoreontologies.org/ont00000898>
                <https://www.commoncoreontologies.org/ont00000917>
                <https://www.commoncoreontologies.org/ont00000929>
                <https://www.commoncoreontologies.org/ont00000984>
                <https://www.commoncoreontologies.org/ont00000987>
                <https://www.commoncoreontologies.org/ont00001006>
                <https://www.commoncoreontologies.org/ont00001141>
              )
] .


###  Generated by the OWL API (version 4.5.29.2024-05-13T12:11:03Z) https://github.com/owlcs/owlapi
