@prefix : <http://www.semanticweb.org/alecsculley/ontologies/2025/3/untitled-ontology-113/> .
@prefix owl: <http://www.w3.org/2002/07/owl#> .
@prefix rdf: <http://www.w3.org/1999/02/22-rdf-syntax-ns#> .
@prefix xml: <http://www.w3.org/XML/1998/namespace> .
@prefix xsd: <http://www.w3.org/2001/XMLSchema#> .
@prefix rdfs: <http://www.w3.org/2000/01/rdf-schema#> .
@base <http://www.semanticweb.org/alecsculley/ontologies/2025/3/untitled-ontology-113/> .

<http://www.semanticweb.org/alecsculley/ontologies/2025/3/untitled-ontology-113> rdf:type owl:Ontology ;
                                                                                  owl:imports <https://www.commoncoreontologies.org/2024-11-06/CommonCoreOntologiesMerged> .

#################################################################
#    Annotation properties
#################################################################

###  http://www.w3.org/2004/02/skos/core#altLabel
<http://www.w3.org/2004/02/skos/core#altLabel> rdf:type owl:AnnotationProperty .


###  http://www.w3.org/2004/02/skos/core#definition
<http://www.w3.org/2004/02/skos/core#definition> rdf:type owl:AnnotationProperty .


#################################################################
#    Object Properties
#################################################################

###  http://www.semanticweb.org/alecsculley/ontologies/2025/3/untitled-ontology-113/backedBy
:backedBy rdf:type owl:ObjectProperty ;
          rdfs:label "backed by"@en ;
          <http://www.w3.org/2004/02/skos/core#definition> "x backed by y means x is supported, secured, or guaranteed by y, meaning that the value, performance, or repayment of x is underpinned by y."@en .


###  http://www.semanticweb.org/alecsculley/ontologies/2025/3/untitled-ontology-113/issues
:issues rdf:type owl:ObjectProperty ;
        rdfs:label "issues"@en .


###  http://www.semanticweb.org/alecsculley/ontologies/2025/3/untitled-ontology-113/partOf
:partOf rdf:type owl:ObjectProperty ;
        rdfs:label "part of"@en .


###  http://www.semanticweb.org/alecsculley/ontologies/2025/3/untitled-ontology-113/raisedBy
:raisedBy rdf:type owl:ObjectProperty ;
          rdfs:label "raised by"@en ;
          <http://www.w3.org/2004/02/skos/core#definition> "x raised by y means x is some resource, y is some agent, and x has been generated, collected, or acquired through the fundraising or financing efforts of y."@en .


#################################################################
#    Classes
#################################################################

###  http://www.semanticweb.org/alecsculley/ontologies/2025/3/untitled-ontology-113#12-Month_Time_Period
<http://www.semanticweb.org/alecsculley/ontologies/2025/3/untitled-ontology-113#12-Month_Time_Period> rdf:type owl:Class ;
                                                                                                      rdfs:subClassOf :Time_Period ;
                                                                                                      rdfs:label "12-Month Time Period"@en ;
                                                                                                      <http://www.w3.org/2004/02/skos/core#definition> "A continuous span of 12 consecutive months used as a standard benchmark for assessing performance or compliance."@en .


###  http://www.semanticweb.org/alecsculley/ontologies/2025/3/untitled-ontology-113#90-Day_Time_Period
<http://www.semanticweb.org/alecsculley/ontologies/2025/3/untitled-ontology-113#90-Day_Time_Period> rdf:type owl:Class ;
                                                                                                    rdfs:subClassOf :Time_Period ;
                                                                                                    rdfs:label "90-Day Time Period"@en .


###  http://www.semanticweb.org/alecsculley/ontologies/2025/3/untitled-ontology-113/AccreditedInvestorRole
:AccreditedInvestorRole rdf:type owl:Class ;
                        rdfs:subClassOf :Investor_Role ;
                        rdfs:label "Accredited Investor Role"@en .


###  http://www.semanticweb.org/alecsculley/ontologies/2025/3/untitled-ontology-113/Annual_Income
:Annual_Income rdf:type owl:Class ;
               rdfs:label "Annual Income"@en ;
               <http://www.w3.org/2004/02/skos/core#definition> "Annual income is the total amount of money earned or received by an individual or entity over the course of a year, typically including wages, salaries, bonuses, dividends, and other sources of revenue before taxes."@en .


###  http://www.semanticweb.org/alecsculley/ontologies/2025/3/untitled-ontology-113/Asset
:Asset rdf:type owl:Class ;
       rdfs:subClassOf <https://www.commoncoreontologies.org/ont00000740> ;
       rdfs:label "Asset"@en ;
       <http://www.w3.org/2004/02/skos/core#definition> "An Asset is a Resource that has economic value and is expected to generate future financial benefits."@en .


###  http://www.semanticweb.org/alecsculley/ontologies/2025/3/untitled-ontology-113/Bad_Actor
:Bad_Actor rdf:type owl:Class ;
           owl:equivalentClass [ owl:intersectionOf ( <https://www.commoncoreontologies.org/ont00001017>
                                                      [ rdf:type owl:Restriction ;
                                                        owl:onProperty <http://purl.obolibrary.org/obo/BFO_0000196> ;
                                                        owl:someValuesFrom :Bad_Actor_Role
                                                      ]
                                                    ) ;
                                 rdf:type owl:Class
                               ] ;
           rdfs:subClassOf <https://www.commoncoreontologies.org/ont00001017> ;
           rdfs:label "Bad Actor"@en ;
           <http://www.w3.org/2004/02/skos/core#definition> "An agent that is bearer of some bad actor role."@en .


###  http://www.semanticweb.org/alecsculley/ontologies/2025/3/untitled-ontology-113/Bad_Actor_Role
:Bad_Actor_Role rdf:type owl:Class ;
                rdfs:subClassOf <http://purl.obolibrary.org/obo/BFO_0000023> ;
                rdfs:label "Bad Actor Role"@en .


###  http://www.semanticweb.org/alecsculley/ontologies/2025/3/untitled-ontology-113/Blank_Check_Company
:Blank_Check_Company rdf:type owl:Class ;
                     rdfs:subClassOf <https://folio.openlegalstandard.org/RDdgYa5ZbqVnS9aGrOwQu5h> ;
                     rdfs:label "Blank Check Company"@en ;
                     <http://www.w3.org/2004/02/skos/core#definition> "An incorporated organization that lacks a specific busniess plan or identified acquisition, often formed for future mergers or acquisitions."@en .


###  http://www.semanticweb.org/alecsculley/ontologies/2025/3/untitled-ontology-113/Business_Development_Company
:Business_Development_Company rdf:type owl:Class ;
                              rdfs:subClassOf :Registered_Investment_Company ;
                              rdfs:label "Business Development Company"@en ;
                              <http://www.w3.org/2004/02/skos/core#definition> "A registered investment company that invests in or assists small, developing, or financially distressed incorporated organizations."@en .


###  http://www.semanticweb.org/alecsculley/ontologies/2025/3/untitled-ontology-113/Canadian_Issuer
:Canadian_Issuer rdf:type owl:Class ;
                 rdfs:subClassOf :Non-U.S._Issuer ;
                 rdfs:label "Canadian Issuer"@en ;
                 <http://www.w3.org/2004/02/skos/core#definition> "A Canadian Issuer is a non-U.S. Issuer that is incorporated or based in Canada."@en .


###  http://www.semanticweb.org/alecsculley/ontologies/2025/3/untitled-ontology-113/Capital-Raising_Limit
:Capital-Raising_Limit rdf:type owl:Class ;
                       rdfs:label "Capital-Raising Limit"@en .


###  http://www.semanticweb.org/alecsculley/ontologies/2025/3/untitled-ontology-113/DisclosureDocumentContent
:DisclosureDocumentContent rdf:type owl:Class ;
                           rdfs:subClassOf :LegalDocumentContent ;
                           owl:disjointWith :OfferingDocumentContent ;
                           rdfs:label "Disclosure Document Content"@en .


###  http://www.semanticweb.org/alecsculley/ontologies/2025/3/untitled-ontology-113/Disclosure_Document
:Disclosure_Document rdf:type owl:Class ;
                     owl:equivalentClass [ owl:intersectionOf ( :Legal_Document
                                                                [ rdf:type owl:Restriction ;
                                                                  owl:onProperty <http://purl.obolibrary.org/obo/BFO_0000101> ;
                                                                  owl:someValuesFrom :DisclosureDocumentContent
                                                                ]
                                                              ) ;
                                           rdf:type owl:Class
                                         ] ;
                     rdfs:subClassOf :Legal_Document ;
                     rdfs:label "Disclosure Document"@en ;
                     <http://www.w3.org/2004/02/skos/core#definition> "A legal document that is carrier of some disclosure document content."@en .


###  http://www.semanticweb.org/alecsculley/ontologies/2025/3/untitled-ontology-113/Exchange_Act_Reporting_Company
:Exchange_Act_Reporting_Company rdf:type owl:Class ;
                                rdfs:subClassOf <https://folio.openlegalstandard.org/RDdgYa5ZbqVnS9aGrOwQu5h> ;
                                rdfs:label "Exchange Act Reporting Company"@en ;
                                <http://www.w3.org/2004/02/skos/core#definition> "An incorporated organization that is registered under the Securities Exchange Act of 1934 and files periodic reports with the SEC."@en .


###  http://www.semanticweb.org/alecsculley/ontologies/2025/3/untitled-ontology-113/Federal_Limit
:Federal_Limit rdf:type owl:Class ;
               rdfs:subClassOf :Offering_Limit ;
               rdfs:label "Federal Offering Limit"@en .


###  http://www.semanticweb.org/alecsculley/ontologies/2025/3/untitled-ontology-113/Form_C
:Form_C rdf:type owl:Class ;
        rdfs:subClassOf :Disclosure_Document ;
        rdfs:label "Form C"@en ;
        <http://www.w3.org/2004/02/skos/core#definition> "Form C is the disclosure document that an issuer must file with the SEC when conducting a securities offering under Regulation Crowdfunding, detailing the company’s business, financial condition, offering specifics, and intended use of proceeds to inform potential investors."@en .


###  http://www.semanticweb.org/alecsculley/ontologies/2025/3/untitled-ontology-113/General_Solicitation
:General_Solicitation rdf:type owl:Class ;
                      rdfs:subClassOf :Solicitation ;
                      rdfs:label "Act of General Solicitation"@en ;
                      <http://www.w3.org/2004/02/skos/core#definition> "An act of solicitation that targets the public broadly by using mass communication channels."@en .


###  http://www.semanticweb.org/alecsculley/ontologies/2025/3/untitled-ontology-113/In-State_Resident
:In-State_Resident rdf:type owl:Class ;
                   rdfs:subClassOf <https://www.commoncoreontologies.org/ont00001017> ;
                   rdfs:label "In-State Resident"@en ;
                   <http://www.w3.org/2004/02/skos/core#definition> "An In-state Resident is a person or organization that is legally domiciled or primarily located in a particular state, often relevant for intrastate offerings."@en .


###  http://www.semanticweb.org/alecsculley/ontologies/2025/3/untitled-ontology-113/Internet_Platform
:Internet_Platform rdf:type owl:Class ;
                   rdfs:label "Internet Platform"@en ;
                   <http://www.w3.org/2004/02/skos/core#definition> "An internet platform is a digital ecosystem or service accessible online that enables users to interact, exchange information, and conduct transactions through provided tools and applications."@en .


###  http://www.semanticweb.org/alecsculley/ontologies/2025/3/untitled-ontology-113/Investment_Company
:Investment_Company rdf:type owl:Class ;
                    rdfs:subClassOf <https://folio.openlegalstandard.org/RDdgYa5ZbqVnS9aGrOwQu5h> ;
                    rdfs:label "Investment Company"@en ;
                    <http://www.w3.org/2004/02/skos/core#definition> "An incorporated organization whose principal activity involves investing, holding, or trading securities."@en .


###  http://www.semanticweb.org/alecsculley/ontologies/2025/3/untitled-ontology-113/Investment_Limit
:Investment_Limit rdf:type owl:Class ;
                  rdfs:subClassOf :Capital-Raising_Limit ;
                  rdfs:label "Investment Limit"@en .


###  http://www.semanticweb.org/alecsculley/ontologies/2025/3/untitled-ontology-113/Investor_Role
:Investor_Role rdf:type owl:Class ;
               rdfs:subClassOf <http://purl.obolibrary.org/obo/BFO_0000023> ;
               rdfs:label "Investor Role"@en .


###  http://www.semanticweb.org/alecsculley/ontologies/2025/3/untitled-ontology-113/Issuer_Role
:Issuer_Role rdf:type owl:Class ;
             rdfs:subClassOf <http://purl.obolibrary.org/obo/BFO_0000023> ;
             rdfs:label "Issuer Role"@en .


###  http://www.semanticweb.org/alecsculley/ontologies/2025/3/untitled-ontology-113/LegalDocumentContent
:LegalDocumentContent rdf:type owl:Class ;
                      rdfs:subClassOf <https://www.commoncoreontologies.org/ont00000958> ;
                      rdfs:label "Legal Document Content"@en .


###  http://www.semanticweb.org/alecsculley/ontologies/2025/3/untitled-ontology-113/Legal_Document
:Legal_Document rdf:type owl:Class ;
                owl:equivalentClass [ owl:intersectionOf ( <https://www.commoncoreontologies.org/ont00001298>
                                                           [ rdf:type owl:Restriction ;
                                                             owl:onProperty <http://purl.obolibrary.org/obo/BFO_0000101> ;
                                                             owl:someValuesFrom :LegalDocumentContent
                                                           ]
                                                         ) ;
                                      rdf:type owl:Class
                                    ] ;
                rdfs:subClassOf <https://www.commoncoreontologies.org/ont00001298> ;
                rdfs:label "Legal Document"@en ;
                <http://www.w3.org/2004/02/skos/core#definition> "A document that is carrier of some legal document content."@en .


###  http://www.semanticweb.org/alecsculley/ontologies/2025/3/untitled-ontology-113/Net_Worth
:Net_Worth rdf:type owl:Class ;
           rdfs:label "Net Worth"@en ;
           <http://www.w3.org/2004/02/skos/core#definition> "Net worth is defined as the total value of an individual’s or entity’s assets minus their total liabilities, representing their overall financial position or wealth."@en .


###  http://www.semanticweb.org/alecsculley/ontologies/2025/3/untitled-ontology-113/Non-Accredited_Investor
:Non-Accredited_Investor rdf:type owl:Class ;
                         owl:equivalentClass [ owl:intersectionOf ( <https://folio.openlegalstandard.org/R8hWq9dSn0Su2Y59JE48V3H>
                                                                    [ rdf:type owl:Class ;
                                                                      owl:complementOf [ rdf:type owl:Restriction ;
                                                                                         owl:onProperty <http://purl.obolibrary.org/obo/BFO_0000196> ;
                                                                                         owl:someValuesFrom :AccreditedInvestorRole
                                                                                       ]
                                                                    ]
                                                                  ) ;
                                               rdf:type owl:Class
                                             ] ;
                         rdfs:subClassOf <https://folio.openlegalstandard.org/R8hWq9dSn0Su2Y59JE48V3H> ;
                         owl:disjointWith <https://folio.openlegalstandard.org/RCwEVoFW90PLN1eL6JToOMt> ;
                         rdfs:label "Non-Accredited Investor"@en ;
                         <http://www.w3.org/2004/02/skos/core#definition> "An investor and is not bearer of some accredited investor role."@en .


###  http://www.semanticweb.org/alecsculley/ontologies/2025/3/untitled-ontology-113/Non-U.S._Issuer
:Non-U.S._Issuer rdf:type owl:Class ;
                 rdfs:subClassOf <https://folio.openlegalstandard.org/RDM4k8t0O3hy93vQwQzEcpg> ;
                 rdfs:label "Non-U.S. Issuer"@en ;
                 <http://www.w3.org/2004/02/skos/core#definition> "A non-U.S. Issuer is an Issuer that is organized or primarily based outside the United States."@en .


###  http://www.semanticweb.org/alecsculley/ontologies/2025/3/untitled-ontology-113/Offeree
:Offeree rdf:type owl:Class ;
         owl:equivalentClass [ owl:intersectionOf ( <https://www.commoncoreontologies.org/ont00001017>
                                                    [ rdf:type owl:Restriction ;
                                                      owl:onProperty <http://purl.obolibrary.org/obo/BFO_0000196> ;
                                                      owl:someValuesFrom :Offeree_Role
                                                    ]
                                                  ) ;
                               rdf:type owl:Class
                             ] ;
         rdfs:subClassOf <https://www.commoncoreontologies.org/ont00001017> ;
         rdfs:label "Offeree"@en ;
         <http://www.w3.org/2004/02/skos/core#definition> "An Offeree is a prospective investor to whom an Issuer extends an offer to purchase securities."@en .


###  http://www.semanticweb.org/alecsculley/ontologies/2025/3/untitled-ontology-113/Offeree_Role
:Offeree_Role rdf:type owl:Class ;
              rdfs:subClassOf <http://purl.obolibrary.org/obo/BFO_0000023> ;
              rdfs:label "Offeree Role"@en .


###  http://www.semanticweb.org/alecsculley/ontologies/2025/3/untitled-ontology-113/OfferingDocumentContent
:OfferingDocumentContent rdf:type owl:Class ;
                         rdfs:subClassOf :LegalDocumentContent ;
                         rdfs:label "Offering Document Content"@en ;
                         <http://www.w3.org/2004/02/skos/core#definition> "An Offering Document is a comprehensive legal document provided by a company or financial entity to potential investors, detailing the terms, conditions, and risks of the investment offering. This document, often used in private placements and public offerings, includes key information such as the company's business model, financial statements, management background, and details of the security being offered."@en .


###  http://www.semanticweb.org/alecsculley/ontologies/2025/3/untitled-ontology-113/Offering_Limit
:Offering_Limit rdf:type owl:Class ;
                rdfs:subClassOf :Capital-Raising_Limit ;
                rdfs:label "Offering Limit"@en ;
                <http://www.w3.org/2004/02/skos/core#definition> "An Offering Limit is a regulatory cap on the total amount of capital that can be raised under a particular exemption within a specified timeframe."@en .


###  http://www.semanticweb.org/alecsculley/ontologies/2025/3/untitled-ontology-113/Process_of_Issuing_Securities
:Process_of_Issuing_Securities rdf:type owl:Class ;
                               rdfs:subClassOf <https://www.commoncoreontologies.org/ont00001314> ;
                               rdfs:label "Act of Issuing Securities"@en ;
                               <http://www.w3.org/2004/02/skos/core#definition> "A legal system act in which an agent creates, registers, and offers its financial instruments to investors."@en .


###  http://www.semanticweb.org/alecsculley/ontologies/2025/3/untitled-ontology-113/Process_of_Testing_the_Waters
:Process_of_Testing_the_Waters rdf:type owl:Class ;
                               rdfs:subClassOf <https://www.commoncoreontologies.org/ont00000402> ;
                               rdfs:label "Act of Testing the Waters"@en ;
                               <http://www.w3.org/2004/02/skos/core#definition> "An act of communication in which an issuer engages potential investors before formally committing to an offering."@en .


###  http://www.semanticweb.org/alecsculley/ontologies/2025/3/untitled-ontology-113/Process_of_Transaction
:Process_of_Transaction rdf:type owl:Class ;
                        rdfs:subClassOf <https://www.commoncoreontologies.org/ont00000228> ;
                        rdfs:label "Act of Transacting"@en ;
                        <http://www.w3.org/2004/02/skos/core#definition> "A planned act in which agents exchange entities of economic value."@en .


###  http://www.semanticweb.org/alecsculley/ontologies/2025/3/untitled-ontology-113/Qualification
:Qualification rdf:type owl:Class ;
               rdfs:subClassOf <https://www.commoncoreontologies.org/ont00001314> ;
               rdfs:label "Act of Qualificaiton"@en ;
               <http://www.w3.org/2004/02/skos/core#altLabel> "Qualification"@en ;
               <http://www.w3.org/2004/02/skos/core#definition> "A legal system act in which a securities authority declares that an offering document meets the legal requirements."@en .


###  http://www.semanticweb.org/alecsculley/ontologies/2025/3/untitled-ontology-113/Raised_Capital
:Raised_Capital rdf:type owl:Class ;
                rdfs:subClassOf <https://folio.openlegalstandard.org/RxkTKgYqWS0WBHnJgrn27Y> ;
                rdfs:label "Raised Capital"@en ;
                <http://www.w3.org/2004/02/skos/core#definition> "A financial asset a company secures by issuing securities to external investors, which then become part of its capital for operations and growth."@en .


###  http://www.semanticweb.org/alecsculley/ontologies/2025/3/untitled-ontology-113/Registered_Intermediary
:Registered_Intermediary rdf:type owl:Class ;
                         owl:equivalentClass [ owl:intersectionOf ( <https://www.commoncoreontologies.org/ont00001017>
                                                                    [ rdf:type owl:Restriction ;
                                                                      owl:onProperty <http://purl.obolibrary.org/obo/BFO_0000196> ;
                                                                      owl:someValuesFrom :Registered_Intermediary_Role
                                                                    ]
                                                                  ) ;
                                               rdf:type owl:Class
                                             ] ;
                         rdfs:subClassOf <https://www.commoncoreontologies.org/ont00001017> ;
                         rdfs:label "Registered Intermediary"@en ;
                         <http://www.w3.org/2004/02/skos/core#definition> "A registered intermediary is an individual or firm that has been formally registered with a regulatory authority to act as a trusted agent between parties—such as issuers and investors—in financial transactions, ensuring compliance with applicable laws and regulations."@en .


###  http://www.semanticweb.org/alecsculley/ontologies/2025/3/untitled-ontology-113/Registered_Intermediary_Role
:Registered_Intermediary_Role rdf:type owl:Class ;
                              rdfs:subClassOf <http://purl.obolibrary.org/obo/BFO_0000023> ;
                              rdfs:label "Registered Intermediary Role"@en .


###  http://www.semanticweb.org/alecsculley/ontologies/2025/3/untitled-ontology-113/Registered_Investment_Company
:Registered_Investment_Company rdf:type owl:Class ;
                               rdfs:subClassOf :Investment_Company ;
                               rdfs:label "Registered Investment Company"@en ;
                               <http://www.w3.org/2004/02/skos/core#definition> "An investment company that has formally registered under the Investment Company Act of 1940."@en .


###  http://www.semanticweb.org/alecsculley/ontologies/2025/3/untitled-ontology-113/Security
:Security rdf:type owl:Class ;
          rdfs:subClassOf <https://folio.openlegalstandard.org/RxkTKgYqWS0WBHnJgrn27Y> ;
          rdfs:label "Security"@en ;
          <http://www.w3.org/2004/02/skos/core#definition> "A financial asset that represents an ownership interest, creditor relationship, or rights to potential future value."@en .


###  http://www.semanticweb.org/alecsculley/ontologies/2025/3/untitled-ontology-113/Solicitation
:Solicitation rdf:type owl:Class ;
              rdfs:subClassOf <https://www.commoncoreontologies.org/ont00000402> ,
                              [ rdf:type owl:Restriction ;
                                owl:onProperty :partOf ;
                                owl:someValuesFrom :Process_of_Issuing_Securities
                              ] ;
              rdfs:label "Act of Solicitation"@en ;
              <http://www.w3.org/2004/02/skos/core#definition> "An act of communication in which an issuer, or agent of an issuer, seeks to attract potential investors to purchase securities."@en .


###  http://www.semanticweb.org/alecsculley/ontologies/2025/3/untitled-ontology-113/Sophisticated_Investor
:Sophisticated_Investor rdf:type owl:Class ;
                        rdfs:subClassOf <https://folio.openlegalstandard.org/R8hWq9dSn0Su2Y59JE48V3H> ;
                        rdfs:label "Sophisticated Investor"@en ;
                        <http://www.w3.org/2004/02/skos/core#definition> "A Sophisticated Investor is an Investor possessing sufficient knowledge and experience to evaluate the risks and merits of an offering, but may not meet accredited thresholds."@en .


###  http://www.semanticweb.org/alecsculley/ontologies/2025/3/untitled-ontology-113/State_Limit
:State_Limit rdf:type owl:Class ;
             rdfs:subClassOf :Offering_Limit ;
             rdfs:label "State Offering Limit"@en .


###  http://www.semanticweb.org/alecsculley/ontologies/2025/3/untitled-ontology-113/Time_Period
:Time_Period rdf:type owl:Class ;
             rdfs:subClassOf <http://purl.obolibrary.org/obo/BFO_0000202> ;
             rdfs:label "Time Period"@en ;
             <http://www.w3.org/2004/02/skos/core#definition> "A defined interval during which a particular event occurs."@en .


###  http://www.semanticweb.org/alecsculley/ontologies/2025/3/untitled-ontology-113/U.S._Issuer
:U.S._Issuer rdf:type owl:Class ;
             rdfs:subClassOf <https://folio.openlegalstandard.org/RDM4k8t0O3hy93vQwQzEcpg> ;
             rdfs:label "U.S. Issuer"@en ;
             <http://www.w3.org/2004/02/skos/core#definition> "A U.S. Issuer is an Issuer that is organized or maintains its principal place of business in the United States."@en .


###  https://folio.openlegalstandard.org/R8hWq9dSn0Su2Y59JE48V3H
<https://folio.openlegalstandard.org/R8hWq9dSn0Su2Y59JE48V3H> rdf:type owl:Class ;
                                                              owl:equivalentClass [ owl:intersectionOf ( <https://www.commoncoreontologies.org/ont00001017>
                                                                                                         [ rdf:type owl:Restriction ;
                                                                                                           owl:onProperty <http://purl.obolibrary.org/obo/BFO_0000196> ;
                                                                                                           owl:someValuesFrom :Investor_Role
                                                                                                         ]
                                                                                                       ) ;
                                                                                    rdf:type owl:Class
                                                                                  ] ;
                                                              rdfs:subClassOf <https://www.commoncoreontologies.org/ont00001017> ;
                                                              rdfs:label "Investor"@en ;
                                                              <http://www.w3.org/2004/02/skos/core#definition> "An agent that is bearer of some investor role."@en .


###  https://folio.openlegalstandard.org/RBGd796pNg5ltGWhkyk2ifm
<https://folio.openlegalstandard.org/RBGd796pNg5ltGWhkyk2ifm> rdf:type owl:Class ;
                                                              owl:equivalentClass [ owl:intersectionOf ( :Security
                                                                                                         [ rdf:type owl:Restriction ;
                                                                                                           owl:onProperty :backedBy ;
                                                                                                           owl:someValuesFrom :Asset
                                                                                                         ]
                                                                                                       ) ;
                                                                                    rdf:type owl:Class
                                                                                  ] ;
                                                              rdfs:subClassOf :Security ;
                                                              rdfs:label "Asset-Backed Security"@en ;
                                                              <http://www.w3.org/2004/02/skos/core#definition> "A security backed by some asset."@en .


###  https://folio.openlegalstandard.org/RCwEVoFW90PLN1eL6JToOMt
<https://folio.openlegalstandard.org/RCwEVoFW90PLN1eL6JToOMt> rdf:type owl:Class ;
                                                              owl:equivalentClass [ owl:intersectionOf ( <https://folio.openlegalstandard.org/R8hWq9dSn0Su2Y59JE48V3H>
                                                                                                         [ rdf:type owl:Restriction ;
                                                                                                           owl:onProperty <http://purl.obolibrary.org/obo/BFO_0000196> ;
                                                                                                           owl:someValuesFrom :AccreditedInvestorRole
                                                                                                         ]
                                                                                                       ) ;
                                                                                    rdf:type owl:Class
                                                                                  ] ;
                                                              rdfs:subClassOf <https://folio.openlegalstandard.org/R8hWq9dSn0Su2Y59JE48V3H> ;
                                                              rdfs:label "Accredited Investor"@en ;
                                                              <http://www.w3.org/2004/02/skos/core#definition> "An investor that is bearer of some accredited investor role."@en .


###  https://folio.openlegalstandard.org/RDM4k8t0O3hy93vQwQzEcpg
<https://folio.openlegalstandard.org/RDM4k8t0O3hy93vQwQzEcpg> rdf:type owl:Class ;
                                                              owl:equivalentClass [ owl:intersectionOf ( <https://www.commoncoreontologies.org/ont00001017>
                                                                                                         [ rdf:type owl:Restriction ;
                                                                                                           owl:onProperty <http://purl.obolibrary.org/obo/BFO_0000196> ;
                                                                                                           owl:someValuesFrom :Issuer_Role
                                                                                                         ]
                                                                                                       ) ;
                                                                                    rdf:type owl:Class
                                                                                  ] ;
                                                              rdfs:subClassOf <https://www.commoncoreontologies.org/ont00001017> ;
                                                              rdfs:label "Issuer"@en ;
                                                              <http://www.w3.org/2004/02/skos/core#definition> "An issuer is a legal entity that develops, registers and sells securities to finance its operations. Issuers may be corporations, investment trusts, or domestic or foreign governments."@en .


###  https://folio.openlegalstandard.org/RDdgYa5ZbqVnS9aGrOwQu5h
<https://folio.openlegalstandard.org/RDdgYa5ZbqVnS9aGrOwQu5h> rdf:type owl:Class ;
                                                              owl:equivalentClass <https://www.commoncoreontologies.org/ont00000010> ;
                                                              rdfs:subClassOf <https://www.commoncoreontologies.org/ont00001180> ;
                                                              rdfs:label "Corporation"@en ;
                                                              <http://www.w3.org/2004/02/skos/core#altLabel> "Company"@en ;
                                                              <http://www.w3.org/2004/02/skos/core#definition> "An organization formed with state governmental approval to act as an artificial person that is empowered with legal rights usually only reserved for individuals, such as to sue and be sued, issue shares of stock to raise funds (unless it is non-profit), own property, hire employees or loan and borrow money."@en .


###  https://folio.openlegalstandard.org/RFLCbWnBgkHxPAEeVWloyg
<https://folio.openlegalstandard.org/RFLCbWnBgkHxPAEeVWloyg> rdf:type owl:Class ;
                                                             rdfs:subClassOf <https://www.commoncoreontologies.org/ont00001314> ;
                                                             rdfs:label "Act of Filing"@en ;
                                                             <http://www.w3.org/2004/02/skos/core#definition> "A legal system act that consists in the submission of a legal document that initiates some legal system act."@en .


###  https://folio.openlegalstandard.org/RmqysGFQ1RYW3F9lv5u3hu
<https://folio.openlegalstandard.org/RmqysGFQ1RYW3F9lv5u3hu> rdf:type owl:Class ;
                                                             rdfs:subClassOf :Legal_Document ;
                                                             rdfs:label "Offering Document"@en ;
                                                             <http://www.w3.org/2004/02/skos/core#altLabel> "Offering Statement"@en ;
                                                             <http://www.w3.org/2004/02/skos/core#definition> "A legal document that is carrier of some offering document content."@en .


###  https://folio.openlegalstandard.org/RxkTKgYqWS0WBHnJgrn27Y
<https://folio.openlegalstandard.org/RxkTKgYqWS0WBHnJgrn27Y> rdf:type owl:Class ;
                                                             rdfs:subClassOf :Asset ;
                                                             rdfs:label "Financial Asset"@en ;
                                                             <http://www.w3.org/2004/02/skos/core#altLabel> "Capital Resource"@en ;
                                                             <http://www.w3.org/2004/02/skos/core#definition> "An asset that has financial value, and which is expected to generate future financial benefits."@en .


###  https://www.commoncoreontologies.org/ont00000740
<https://www.commoncoreontologies.org/ont00000740> rdf:type owl:Class ;
                                                   rdfs:label "Resource"@en ;
                                                   <http://www.w3.org/2004/02/skos/core#definition> "A Continuant that is owned by, in the possession of, or is otherwise controlled by an Agent such that it could be used by that Agent."@en .


#################################################################
#    General axioms
#################################################################

[ rdf:type owl:AllDisjointClasses ;
  owl:members ( :Bad_Actor_Role
                :Investor_Role
                :Issuer_Role
                :Offeree_Role
                :Registered_Intermediary_Role
                <https://www.commoncoreontologies.org/ont00000038>
                <https://www.commoncoreontologies.org/ont00000173>
                <https://www.commoncoreontologies.org/ont00000175>
                <https://www.commoncoreontologies.org/ont00000187>
                <https://www.commoncoreontologies.org/ont00000392>
                <https://www.commoncoreontologies.org/ont00000485>
                <https://www.commoncoreontologies.org/ont00000506>
                <https://www.commoncoreontologies.org/ont00000599>
                <https://www.commoncoreontologies.org/ont00000758>
                <https://www.commoncoreontologies.org/ont00000898>
                <https://www.commoncoreontologies.org/ont00000917>
                <https://www.commoncoreontologies.org/ont00000929>
                <https://www.commoncoreontologies.org/ont00000984>
                <https://www.commoncoreontologies.org/ont00000987>
                <https://www.commoncoreontologies.org/ont00001006>
                <https://www.commoncoreontologies.org/ont00001141>
              )
] .


###  Generated by the OWL API (version 4.5.29.2024-05-13T12:11:03Z) https://github.com/owlcs/owlapi
